src/inductive/inductive_graph_measure.v
@@ -18,114 +18,105 @@ Require Import GraphVerification.src.util.util.
 Require Import GraphVerification.src.util.NatMap.
 Require Import GraphVerification.src.inductive.inductive_graph.
 
+(* Stating and proving Lemmas and Theorems about measuring the size of an IG.
+These are the only proofs that the last remaining computational functions on IGs need to prove termination.
+*)
+
+(* Lemmas and Theorems try to have only the context as an argument, and break it up internally, and this allows proof to do this too *)
+Ltac destruct_context c := destruct c as [[[froms node] label] tos].
 
 
 Lemma IG_labNodes_len_cardinal : forall (A B : Type) (ig : IG A B),
-    NatMap.cardinal ig = IG_noNodes ig.
+    IG_noNodes ig = NatMap.cardinal ig.
 Proof.
     intros. unfold IG_noNodes. unfold IG_labNodes. rewrite map_length.
     rewrite NatMap.cardinal_1. reflexivity. 
 Qed.
 
-Lemma IG_match_returns_node : forall (A B : Type) (query hit : Node) (ig i : IG A B) (froms tos : Adj B) (l : A),
-    IG_match query ig = (Some (froms, hit, l, tos), i) -> query = hit.
+Lemma IG_match_returns_node : forall (A B : Type) (query : Node) (c : Context A B) (ig i : IG A B),
+    IG_match query ig = (Some c, i) -> let '(_, hit, _, _) := c in query = hit.
 Proof.
-    intros. unfold IG_match in H. destruct (NatMap.find query ig).
-    - unfold _cleanSplit in H. destruct c as [[fromss label] toss]. inversion H. reflexivity. 
+    destruct_context c. intros. unfold IG_match in H. destruct (NatMap.find query ig).
+    - unfold _cleanSplit in H. destruct c as [[fromss labell] toss]. inversion H. reflexivity. 
     - inversion H.
 Qed.
 
 
 Lemma IG_match_none_returns_graph : forall (A B : Type) (query : Node) (ig i : IG A B),
-  IG_match query ig = (None, i) -> ig = i.
+    IG_match query ig = (None, i) -> ig = i.
 Proof.
-  intros. unfold IG_match in H. destruct (NatMap.find query ig).
-  - destruct (_cleanSplit query c (NatMap.remove query ig)). inversion H.
-  - inversion H. reflexivity.
+    intros. unfold IG_match in H. destruct (NatMap.find query ig).
+    - destruct (_cleanSplit query c (NatMap.remove query ig)). inversion H.
+    - inversion H. reflexivity.
 Qed.
-
 
 
 
 Lemma _IG_updateEntry_does_not_change_cardinality : forall {A B : Type} (node : Node) (f : Context' A B -> Context' A B) (ig : IG A B), 
     NatMap.cardinal (_updateEntry node f ig) = NatMap.cardinal ig.
 Proof.
-  intros. unfold _updateEntry.
+    intros. unfold _updateEntry.
 
-  destruct (NatMap.find node ig) eqn:split.
-  - 
-
-  assert (NatMap.Equal ig (NatMap.add node c ig)). { 
-      apply MFacts.find_mapsto_iff in split.
-
-    apply MFacts.Equal_mapsto_iff.
-    split; intros.
-    - apply MFacts.add_mapsto_iff.
-       bdestruct (node =? k).
-      + subst. left. split.
-      -- reflexivity.
-      -- apply MFacts.find_mapsto_iff in split. apply MFacts.find_mapsto_iff in H. rewrite H in split. inversion split. reflexivity.
-      + right. split.
-      -- assumption.
-      -- assumption.
-    - apply MFacts.add_mapsto_iff in H. destruct H.
-      + destruct H. subst. assumption.
-      + destruct H. assumption.
-  }
-  rewrite H at 2.
-  apply NatMap_add_value_does_not_matter_for_cardinality.
-  - reflexivity.
+    destruct (NatMap.find node ig) eqn:split.
+    - apply NatMap_find_some_add_some_idem in split.
+        rewrite split at 2.
+        apply NatMap_add_value_does_not_matter_for_cardinality.
+    - reflexivity.
 Qed.
-
 
 
 Lemma _IG_updAdj_does_not_change_cardinality : forall {A B : Type} (adj : Adj B) (f : B -> Context' A B -> Context' A B) (ig : IG A B), 
     NatMap.cardinal (_updAdj adj f ig) = NatMap.cardinal ig.
 Proof.
-  intros.
-  unfold _updAdj.
-  induction adj.
-  - simpl. reflexivity.
-  - simpl. rewrite <- IHadj.
-    pose proof (@_IG_updateEntry_does_not_change_cardinality A B).
-    destruct a.
-    rewrite H. reflexivity.
+    intros.
+    unfold _updAdj.
+    induction adj; simpl.
+    - reflexivity.
+    - rewrite <- IHadj. destruct a.
+        rewrite _IG_updateEntry_does_not_change_cardinality. reflexivity.
 Qed.
 
 
+Lemma _IG_match_minusOnes_cardinality : forall (A B : Type) (n : Node) (c : Context A B) (ig rest : IG A B),
+    IG_match n ig = (Some c, rest) -> NatMap.cardinal ig = S (NatMap.cardinal rest).
+Proof.
+    intros.
+    apply IG_match_returns_node in H as s. destruct_context c. subst.
+    unfold IG_match in H. destruct (NatMap.find node ig) eqn:find.
+    - destruct (_cleanSplit node c (NatMap.remove node ig)) eqn:split.
+        inversion H. subst.
+        unfold _cleanSplit in split.
+        destruct c as [[fromss labell] toss].
+        inversion split.
+        clear split H1.
+
+        rewrite !_IG_updAdj_does_not_change_cardinality.
+        apply symmetry.
+        apply NatMap_map_find_some_remove_minusOnes_cardinality.
+
+        exists (fromss, labell, toss).
+        apply find.
+    - inversion H.
+Qed.
+
+
+
+Lemma _IG_match_minusOnes_IGnoNodes : forall (A B : Type) (n : Node) (c : Context A B) (ig rest : IG A B),
+    IG_match n ig = (Some c, rest) -> IG_noNodes ig = S (IG_noNodes rest).
+Proof.
+    intros. apply _IG_match_minusOnes_cardinality in H.
+    rewrite !IG_labNodes_len_cardinal.
+    assumption.
+Qed.
 
 
 
 Theorem _IG_match_decreases_IG_noNodes : forall (A B : Type) (n : Node) (c : Context A B) (ig rest : IG A B),
     IG_match n ig = (Some c, rest) -> IG_noNodes rest < IG_noNodes ig.
 Proof.
-    intros. destruct c as [[[froms node] label] tos]. apply IG_match_returns_node in H as s. subst.
-    assert (NatMap.cardinal ig = S (NatMap.cardinal rest)). {
-
-        unfold IG_match in H.
-        destruct (NatMap.find node ig) eqn:split.
-        - destruct (_cleanSplit node c (NatMap.remove node ig)) eqn:split0.
-            inversion H. subst.
-            unfold _cleanSplit in split0.
-            destruct c as [[fromss labell] toss].
-            inversion split0.
-            clear split0 H1.
-            
-
-
-            rewrite _IG_updAdj_does_not_change_cardinality.
-            rewrite _IG_updAdj_does_not_change_cardinality.
-            apply symmetry.
-            apply NatMap_map_find_some_remove_lowers_cardinality.
-
-            exists (fromss, labell, toss).
-            apply split.
-        - inversion H.
-    }
-    rewrite <- !IG_labNodes_len_cardinal.
-    lia.
+    intros.
+    apply _IG_match_minusOnes_IGnoNodes in H. lia.
 Qed.
-
 
 
 Theorem _IG_matchAny_decreases_IG_noNodes : forall (A B : Type) (c : Context A B) (ig rest : IG A B),
